Proved that tree_rep_has_children using path-counting flow interface.

concurrency/verif_bst_flows.v
@@ -56,25 +56,37 @@ Proof.
   intros. exfalso; auto.
 Qed.
 
+Lemma val_eqb_refl: forall x, val_eqb x x = true.
+Proof. intros. now rewrite val_eqb_true. Qed.
+
 Definition edgeFn (x y: TreeNode): nat -> nat :=
-  fun v => if ((negb (val_eqb y.(addr_tn) nullval)) &&
+  fun v => if ((negb (val_eqb x.(addr_tn) y.(addr_tn))) &&
+               (negb (val_eqb y.(addr_tn) nullval)) &&
                ((val_eqb y.(addr_tn) x.(left_tn)) ||
                 (val_eqb y.(addr_tn) x.(right_tn))))%bool then v else O.
+
+Definition address_in (n: TreeNode) (I: pc_flowint): Prop :=
+  exists t, t ∈ domm I /\ addr_tn n = addr_tn t.
+
+Lemma address_not_in_domm: forall n I, ~ address_in n I -> n ∉ domm I.
+Proof. repeat intro. apply H. red. exists n. split; auto. Qed.
 
 Definition global_inv (Ipc: pc_flowint) (root: TreeNode) (NS: list TreeNode): Prop :=
   ✓Ipc /\ (forall n, n ∈ domm Ipc -> n <> root -> inf Ipc n = O) /\
   (inf Ipc root = 1%nat) /\ (In root NS) /\
-  (forall n, n ∉ domm Ipc -> out Ipc n = O) /\ (domm Ipc = list_to_set NS).
+  (forall n, ~ address_in n Ipc -> out Ipc n = O) /\ (domm Ipc = list_to_set NS).
 
-Definition single_inv (t: TreeNode) (It: pc_flowint): Prop :=
+Definition local_inv (t: TreeNode) (It: pc_flowint): Prop :=
   Int.min_signed <= t.(key_tn) <= Int.max_signed /\
+  t.(addr_tn) ≠ t.(left_tn) /\
+  t.(addr_tn) ≠ t.(right_tn) /\
   tc_val (tptr Tvoid) t.(value_tn) /\
   ✓ It /\ inf It t = 1%nat /\
-  (forall n, n ≠ t -> out It n = edgeFn t n 1%nat) /\
+  (forall n, out It n = edgeFn t n 1%nat) /\
   domm It = {[t]}.
 
 Definition node_rep (t: TreeNode) (It: pc_flowint): mpred :=
-  !! single_inv t It &&
+  !! local_inv t It &&
   data_at Tsh t_struct_tree (Vint (Int.repr t.(key_tn)),
                              (t.(value_tn), (t.(left_tn), t.(right_tn)))) t.(addr_tn).
 
@@ -82,13 +94,13 @@ Definition tree_rep (root: TreeNode) (l: list (TreeNode * pc_flowint)): mpred :=
   !! (exists C, list_join (map snd l) C /\ global_inv C root (map fst l)) &&
   iter_sepcon (fun x => node_rep x.1 x.2) l.
 
-Lemma tree_rep_single_inv: forall root l,
-    tree_rep root l |-- !!(forall x, In x l -> single_inv x.1 x.2).
+Lemma tree_rep_local_inv: forall root l,
+    tree_rep root l |-- !!(forall x, In x l -> local_inv x.1 x.2).
 Proof.
   intros. unfold tree_rep. Intros. clear H. induction l.
   - apply prop_right. intros. inversion H.
   - simpl.
-    assert_PROP (forall x, In x l -> single_inv x.1 x.2). {
+    assert_PROP (forall x, In x l -> local_inv x.1 x.2). {
       sep_apply IHl. Intros. apply prop_right. auto. }
     unfold node_rep at 1. Intros. apply prop_right. intros. destruct H1; auto.
     now subst.
@@ -197,16 +209,18 @@ Proof.
   - eapply IHl; eauto.
 Qed.
 
-Lemma tree_rep_no_dangling_node: forall root l,
+Lemma tree_rep_has_parent: forall root l,
     tree_rep root l |--
-             !!(forall x, In x (map fst l) -> x <> root ->
-                          exists p, p.(left_tn) = x.(addr_tn) \/
-                                    p.(right_tn) = x.(addr_tn)).
+             !!(forall x, In x (map fst l) -> x ≠ root ->
+                          x.(addr_tn) ≠ nullval /\
+                          exists p, In p (map fst l) /\ p ≠ x /\
+                                    (p.(left_tn) = x.(addr_tn) \/
+                                     p.(right_tn) = x.(addr_tn))).
 Proof.
-  intros. sep_apply tree_rep_single_inv. Intros. unfold tree_rep. Intros.
+  intros. sep_apply tree_rep_local_inv. Intros. unfold tree_rep. Intros.
   apply prop_right. intros. destruct H0 as [C [? ?]].
   destruct (In_fst_pair _ _ H1) as [y ?]. pose proof (H _ H4). simpl in H5.
-  destruct H5 as [? [? [? [? [? ?]]]]]. rename H4 into Hp.
+  destruct H5 as [? [_ [_ [? [? [? [? ?]]]]]]]. rename H4 into Hp.
   pose proof (In_pair_snd _ _ _ Hp).
   destruct (list_join_single _ _ _ H4 H0) as [[? ?] | [l1 [l2 [z [? [? ?]]]]]].
   - subst C. destruct H3 as [? [? [? [? _]]]]. clear -H14 H1 H11 H2. exfalso.
@@ -240,16 +254,140 @@ Proof.
       destruct H26; auto. right. now right. } apply sum_0or1_1 in H25.
     + destruct H25 as [y0 [? ?]]. specialize (H26 _ H25). apply In_snd_pair in H26.
       destruct H26 as [x0 ?]. specialize (H _ H26). simpl in H.
-      destruct H as [_ [_ [_ [_ [? _]]]]]. rewrite H in H27.
-      * exists x0. clear -H27. unfold edgeFn in H27.
-        match goal with | H: context [match ?E with _ => _ end] |- _ =>
-                          destruct E eqn:?H in H end. 2: inversion H27.
-        apply andb_prop in H0. destruct H0. apply orb_prop in H0.
-        destruct H0; [left | right]; now apply val_eqb_true in H0.
-      * eapply NoDup_pair_snd; eauto. clear -H11 Hn2 H25. rewrite H11 in Hn2.
-        apply NoDup_remove_2 in Hn2. intro. now subst.
+      destruct H as [_ [_ [_ [_ [_ [_ [? _]]]]]]].
+      assert (Hneq: x ≠ x0). {
+        eapply NoDup_pair_snd; eauto. clear -H11 Hn2 H25. rewrite H11 in Hn2.
+        apply NoDup_remove_2 in Hn2. intro. now subst. } rewrite H in H27; auto.
+      clear -H27 H26 Hneq. unfold edgeFn in H27.
+      match goal with | H: context [match ?E with _ => _ end] |- _ =>
+                        destruct E eqn:?H in H end. 2: inversion H27.
+      apply andb_prop in H0. destruct H0. apply orb_prop in H0.
+      apply andb_prop in H. destruct H. apply negb_true in H1.
+      apply val_eqb_false in H1. split; auto.
+      apply In_pair_fst in H26. exists x0. do 2 (split; auto).
+      destruct H0; [left | right]; now apply val_eqb_true in H0.
     + intros. specialize (H26 _ H27). apply In_snd_pair in H26. destruct H26 as [y0 ?].
-      specialize (H _ H26). simpl in H. destruct H as [_ [_ [_ [_ [? _]]]]].
-      rewrite !H. 1: apply edgeFn_0orv. eapply NoDup_pair_snd; eauto.
-      rewrite H11 in Hn2. apply NoDup_remove_2 in Hn2. intro. now subst.
+      specialize (H _ H26). simpl in H. destruct H as [_ [_ [_ [_ [_ [_ [? _]]]]]]].
+      rewrite !H. apply edgeFn_0orv.
+Qed.
+
+Definition has_child_or_none (x: TreeNode) (child: TreeNode -> val)
+           (l: list TreeNode): Prop :=
+  child x = nullval \/ exists p, In p l /\ p ≠ x /\ child x = p.(addr_tn).
+
+Lemma negb_false: forall b, negb b = false <-> b = true.
+Proof. intros; split; intros; destruct b; simpl in *; auto. Qed.
+
+Lemma edgeFn_x_y_eq_addr: forall x y,
+    addr_tn x = addr_tn y -> edgeFn x y 1 = O.
+Proof.
+  intros. unfold edgeFn.
+  match goal with
+  | |- context [match ?E with _ => _ end] => destruct E eqn:?H end; auto.
+  do 2 (apply andb_prop in H0; destruct H0).
+  apply negb_true in H0. apply val_eqb_false in H0. exfalso. now apply H0.
+Qed.
+
+Lemma ani_dec: forall n I, {address_in n I} + {~ address_in n I}.
+Proof.
+  intros. destruct (in_dec Val.eq (addr_tn n) (map addr_tn (elements (domm I)))).
+  - left. apply in_map_iff in i. destruct i as [x [? ?]].
+    rewrite <- elem_of_list_In in H0. apply elem_of_elements in H0.
+    exists x. split; auto.
+  - right. repeat intro. apply n0. rewrite in_map_iff. destruct H as [t [? ?]].
+    exists t. split; auto. rewrite <- elem_of_list_In. now rewrite elem_of_elements.
+Qed.
+
+Lemma tree_rep_has_children: forall root l,
+    tree_rep root l |--
+             !!(forall x, In x (map fst l) ->
+                          has_child_or_none x left_tn (map fst l) /\
+                          has_child_or_none x right_tn (map fst l)).
+Proof.
+  intros. sep_apply tree_rep_local_inv. Intros. unfold tree_rep. Intros.
+  apply prop_right. intros. destruct H0 as [C [? ?]].
+  destruct (In_fst_pair _ _ H1) as [y ?]. pose proof (H _ H3). simpl in H4.
+  destruct H4 as [? [? [? [? [? [? [? ?]]]]]]]. pose proof (In_pair_snd _ _ _ H3).
+  destruct (list_join_single _ _ _ H12 H0) as [[? ?] | [l1 [l2 [z [? [? ?]]]]]].
+  - subst C. destruct l. 1: simpl in H13; inversion H13. destruct l.
+    2: simpl in H13; inversion H13. destruct p. simpl in *. inversion H13. subst p.
+    clear H13 H12. destruct H1. 2: now exfalso. subst t. clear H H0 H3.
+    destruct H2 as [? [? [? [? [? ?]]]]]. simpl in H2. destruct H2. 2: now exfalso.
+    subst x. split.
+    + destruct (Val.eq root.(left_tn) nullval) as [?H | ?H]; [now left | exfalso].
+      remember (Build_TreeNode (left_tn root) 0 nullval nullval nullval) as n.
+      specialize (H10 n). unfold edgeFn in H10. rewrite Heqn in H10. simpl in H10.
+      rewrite <- Heqn in H10.
+      match goal with | H: context [match ?E with _ => _ end] |- _ =>
+                        destruct E eqn:?H in H end.
+      * assert (~ address_in n y). {
+          repeat intro. destruct H14 as [t [? ?]].  rewrite H11 in H14.
+          apply elem_of_singleton_1 in H14. subst. simpl in H15. auto. }
+        specialize (H3 _ H14). rewrite H3 in H10. easy.
+      * apply andb_false_iff in H13. destruct H13.
+        -- apply andb_false_iff in H13.
+           destruct H13; apply negb_false in H13; apply val_eqb_true in H13; auto.
+        -- rewrite val_eqb_refl in H13. now rewrite orb_true_l in H13.
+    + destruct (Val.eq root.(right_tn) nullval) as [?H | ?H]; [now left | exfalso].
+      remember (Build_TreeNode (right_tn root) 0 nullval nullval nullval) as n.
+      specialize (H10 n). unfold edgeFn in H10. rewrite Heqn in H10. simpl in H10.
+      rewrite <- Heqn in H10.
+      match goal with | H: context [match ?E with _ => _ end] |- _ =>
+                        destruct E eqn:?H in H end.
+      * assert (~ address_in n y). {
+          repeat intro. destruct H14 as [t [? ?]].  rewrite H11 in H14.
+          apply elem_of_singleton_1 in H14. subst. simpl in H15. auto. }
+          specialize (H3 _ H14). rewrite H3 in H10. easy.
+      * apply andb_false_iff in H13. destruct H13.
+        -- apply andb_false_iff in H13.
+           destruct H13; apply negb_false in H13; apply val_eqb_true in H13; auto.
+        -- rewrite val_eqb_refl in H13. now rewrite orb_true_r in H13.
+  - red in H15. destruct H2 as [? [? [? [? [? ?]]]]]. split; red.
+    + destruct (Val.eq x.(left_tn) nullval) as [?H | ?H]; [now left | right].
+      pose proof (intJoin_unfold_out _ _ _ H15 H2).
+      assert (forall n, ~ address_in n C -> 0%nat = (edgeFn x n 1 + out z n)%nat). {
+        intros. specialize (H19 _ H23).
+        specialize (H22 _ (address_not_in_domm _ _ H23)). rewrite H19 in H22.
+        now rewrite H10 in H22. }
+      remember (Build_TreeNode (left_tn x) 0 nullval nullval nullval) as n.
+      destruct (ani_dec n C).
+      * unfold address_in in a. destruct a as [t [? ?]]. rewrite Heqn in H25.
+        simpl in H25. exists t. split; [|split]; auto.
+        -- clear -H24 H20. rewrite H20 in H24.
+           apply elem_of_list_to_set in H24.
+           now apply elem_of_list_In in H24.
+        -- intro. subst; auto.
+      * specialize (H23 _ n0). cut (edgeFn x n 1 = 1)%nat.
+        -- intros. exfalso. rewrite H24 in H23. clear -H23. lia.
+        -- unfold edgeFn.
+           match goal with
+           | |- context [match ?E with _ => _ end] => destruct E eqn:?H end; auto.
+           rewrite Heqn in H24. simpl in H24.
+           rewrite ((proj2 (val_eqb_false (addr_tn x) (left_tn x))) H5) in H24.
+           rewrite ((proj2 (val_eqb_false (left_tn x) nullval)) H21) in H24.
+           rewrite val_eqb_refl in H24. simpl in H24. now exfalso.
+    + destruct (Val.eq x.(right_tn) nullval) as [?H | ?H]; [now left | right].
+      pose proof (intJoin_unfold_out _ _ _ H15 H2).
+      assert (forall n, ~ address_in n C -> 0%nat = (edgeFn x n 1 + out z n)%nat). {
+        intros. specialize (H19 _ H23).
+        specialize (H22 _ (address_not_in_domm _ _ H23)). rewrite H19 in H22.
+        now rewrite H10 in H22. }
+      remember (Build_TreeNode (right_tn x) 0 nullval nullval nullval) as n.
+      destruct (ani_dec n C).
+      * unfold address_in in a. destruct a as [t [? ?]]. rewrite Heqn in H25.
+        simpl in H25. exists t. split; [|split]; auto.
+        -- clear -H24 H20. rewrite H20 in H24.
+           apply elem_of_list_to_set in H24.
+           now apply elem_of_list_In in H24.
+        -- intro. subst; auto.
+      * specialize (H23 _ n0). cut (edgeFn x n 1 = 1)%nat.
+        -- intros. exfalso. rewrite H24 in H23. clear -H23. lia.
+        -- unfold edgeFn.
+           match goal with
+           | |- context [match ?E with _ => _ end] => destruct E eqn:?H end; auto.
+           rewrite Heqn in H24. simpl in H24.
+           rewrite ((proj2 (val_eqb_false (addr_tn x) (right_tn x))) H6) in H24.
+           rewrite ((proj2 (val_eqb_false (right_tn x) nullval)) H21) in H24.
+           rewrite val_eqb_refl in H24. simpl in H24. rewrite orb_true_r in H24.
+           now exfalso.
 Qed.
